src/libs/bslSyntax.sig
@@ -310,6 +310,19 @@ sig
     val bconstii:   int -> int -> term
     val bconstimm:  term -> term
 
+    (* Memory constants (BExp_MemConst: bir_exp_t)
+     *
+     * Notes:
+     *  - bconstmem takes an address type, a value type and a
+     *    list of key-value pairs to build up a finite map
+     *    using FUPDATE and FEMPTY. The address and value
+     *    sizes have to be supported by BIR.
+     *
+     * bconstmem:  int -> int -> (int * int) list -> bir_exp_t
+     *)
+
+    val bconstmem: int -> int -> (int * int) list -> term
+
     (* Den (BExp_Den: bir_exp_t)
      *
      * bden: bir_var_t -> bir_exp_t
